theories/Infra/Lattice.v
@@ -10,32 +10,33 @@ Require Export Containers.OrderedType Setoid Coq.Classes.Morphisms Computable.
 Require Export PartialOrder.
 Require Import EqDec DecSolve.
 
-Class BoundedSemiLattice (A : Type) `{PartialOrder A} := {
-  bottom : A;
-  join : A -> A -> A;
+Class JoinSemiLattice (A : Type) `{PartialOrder A} :=
+  {
+      join : A -> A -> A;
 
-  bottom_least : forall a, poLe bottom a;
+      join_idempotent : forall a, poEq (join a a) a;
+      join_commutative : forall a b, poEq (join a b) (join b a);
+      join_associative : forall a b c, poEq (join (join a b) c) (join a (join b c));
+      join_poLe : forall a b, poLe a (join a b);
 
-  join_idempotent : forall a, poEq (join a a) a;
-  join_commutative : forall a b, poEq (join a b) (join b a);
-  join_associative : forall a b c, poEq (join (join a b) c) (join a (join b c));
-  join_poLe : forall a b, poLe a (join a b);
+      join_respects_eq :> Proper (poEq ==> poEq ==> poEq) join;
+      join_respects_le :> Proper (poLe ==> poLe ==> poLe) join
+  }.
 
-  join_respects_eq :> Proper (poEq ==> poEq ==> poEq) join;
-  join_respects_le :> Proper (poLe ==> poLe ==> poLe) join
-}.
+Class LowerBounded (A : Type) `{PartialOrder A} :=
+  {
+    bottom : A;
+    bottom_least : forall a, poLe bottom a;
+  }.
 
 Infix "⊔" := join (at level 70, no associativity).
 Notation "⊥" := bottom (at level 70, no associativity).
 
-
-Instance pair_boundedsemilattice A B `{BoundedSemiLattice A} `{BoundedSemiLattice B}
-  : BoundedSemiLattice (A * B) := {
-  bottom := (bottom, bottom);
+Instance pair_semilattice A B `{JoinSemiLattice A} `{JoinSemiLattice B}
+  : JoinSemiLattice (A * B) := {
   join x y := (join (fst x) (fst y), join (snd x) (snd y))
 }.
 Proof.
-  - intros [a b]; split; simpl; eapply bottom_least.
   - intros [a b]; split; simpl; eapply join_idempotent.
   - intros [a1 a2] [b1 b2]; split; simpl; eapply join_commutative.
   - intros [a1 a2] [b1 b2] [c1 c2]; split; simpl; eapply join_associative.
@@ -46,19 +47,33 @@ Proof.
       split; eapply join_respects_le; eauto.
 Defined.
 
+Instance pair_boundedsemilattice A B `{LowerBounded A} `{LowerBounded B}
+  : LowerBounded (A * B) := {
+  bottom := (bottom, bottom);
+}.
+Proof.
+  - intros [a b]; split; simpl; eapply bottom_least.
+Defined.
 
-Instance bool_boundedsemilattice
-  : BoundedSemiLattice bool := {
-  bottom := false;
+
+Instance bool_joinsemilattice
+  : JoinSemiLattice bool := {
   join := orb
 }.
 Proof.
-  - intros []; simpl; eauto.
   - intros []; simpl; eauto.
   - intros [] []; simpl; eauto.
   - intros [] [] []; simpl; eauto.
   - intros [] []; simpl; eauto.
   - intros [] [] LE [] [] LE'; simpl in *; eauto.
+Defined.
+
+Instance bool_lowerbounded : LowerBounded bool :=
+  {
+    bottom := false
+  }.
+Proof.
+  intros; econstructor.
 Defined.
 
 Require Import OptionR.
@@ -70,7 +85,7 @@ Definition ojoin A join (x y:option A) :=
   | Some x, Some y => Some (join x y)
   end.
 
-Instance ojoin_poEq A `{BoundedSemiLattice A}
+Instance ojoin_poEq A `{JoinSemiLattice A}
   : Proper (poEq ==> poEq ==> poEq) (ojoin A join).
 Proof.
   unfold Proper, respectful.
@@ -79,7 +94,7 @@ Proof.
   econstructor. rewrite H1, H4. reflexivity.
 Qed.
 
-Instance ojoin_poLe A `{BoundedSemiLattice A}
+Instance ojoin_poLe A `{JoinSemiLattice A}
   : Proper (poLe ==> poLe ==> poLe) (ojoin A join).
 Proof.
   unfold Proper, respectful.
@@ -90,188 +105,13 @@ Proof.
   - econstructor. rewrite H3. rewrite H6. reflexivity.
 Qed.
 
-Instance option_boundedsemilattice A `{BoundedSemiLattice A}
-  : @BoundedSemiLattice (option A) (PartialOrder_option_fstNoneOrR _) := {
-  bottom := None;
+Instance option_boundedsemilattice A `{JoinSemiLattice A}
+  : @JoinSemiLattice (option A) (PartialOrder_option_fstNoneOrR _) := {
   join := ojoin _ join
 }.
 Proof.
-  - intros [a|]; simpl; eauto using fstNoneOrR.
   - intros [a|]; simpl; eauto using option_R, join_idempotent.
   - intros [a|] [b|]; simpl; eauto using option_R, join_commutative.
   - intros [a1|] [b1|] [c1|]; simpl; eauto using option_R, join_associative.
   - intros [a|] [b|]; simpl; eauto using fstNoneOrR, join_poLe.
 Defined.
-
-Section SemiLatticeTheory.
-  Variable A : Type.
-  Context `{l : BoundedSemiLattice A}.
-  Hint Immediate join_idempotent join_commutative join_associative.
-
-End SemiLatticeTheory.
-
-(*
-Require Import MoreList.
-
-Instance list_boundedsemilattice A `{BoundedSemiLattice A}
-  : BoundedSemiLattice (list A) := {
-  bottom := nil;
-  join x y := zip join x y
-}.
-Proof.
-  - intros [a b]; split; simpl; eapply bottom_least.
-  - intros [a b]; split; simpl; eapply join_idempotent.
-  - intros [a1 a2] [b1 b2]; split; simpl; eapply join_commutative.
-  - intros [a1 a2] [b1 b2] [c1 c2]; split; simpl; eapply join_associative.
-  - intros [a1 a2] [b1 b2] [EQa EQb] [c1 c2] [d1 d2] [EQc EQd]; simpl in *;
-      split; eapply join_respects_eq; eauto.
-  - intros [a1 a2] [b1 b2] [LEa LEb] [c1 c2] [d1 d2] [LEc LEd]; simpl in *;
-      split; eapply join_respects_le; eauto.
-Defined.
- *)
-
-(*
-Class Lattice (A : Type) `{OrderedType A} := {
-  meet : A -> A -> A;
-  join : A -> A -> A;
-
-  meet_idempotent : forall a, meet a a === a;
-  meet_commutative : forall a b, meet a b === meet b a;
-  meet_associative : forall a b c, meet (meet a b) c === meet a (meet b c);
-  meet_absorptive : forall a b : A, meet a (join a b) === a;
-
-  meet_respects_eq :> Proper (equal ==> _eq ==> _eq) meet;
-  meet_respects_le :> Proper (_le ==> _le ==> _le) meet;
-
-  join_idempotent : forall a, join a a === a;
-  join_commutative : forall a b, join a b === join b a;
-  join_associative : forall a b c, join (join a b) c === join a (join b c);
-  join_absorptive : forall a b : A, join a (meet a b) === a
-
-  join_respects_eq : Proper (_eq ==> _eq ==> _eq) join;
-  join_respects_le : Proper (_le ==> _le ==> _le) join
-}.
-*)
-
-(* Infix "/*\" := meet (at level 40, left associativity) : lattice_scope. *)
-
-
-
-(*
-
-Section LatticeTheory.
-  Context `{l : Lattice A}.
-  Hint Immediate meet_idempotent meet_commutative meet_associative meet_absorptive.
-  Hint Immediate join_idempotent join_commutative join_associative join_absorptive.
-
-  Lemma lte_meet_join : forall a b, a /*\ b === a <-> a \*/ b === b.
-  Proof.
-  split; intro EQ. rewrite <- EQ.
-    rewrite join_commutative.
-    rewrite meet_commutative.
-    rewrite join_absorptive.
-    reflexivity.
-    rewrite meet_absorptive.
-    reflexivity.
-   Qed.
-
-  (** *)
-
-  Definition meet_distributive_l_law := forall x y z, x /*\ (y \*/ z) = (x /*\ y) \*/ (x /*\ z).
-  Definition meet_distributive_r_law := forall x y z, (x \*/ y) /*\ z = (x /*\ z) \*/ (y /*\ z).
-  Definition join_distributive_l_law := forall x y z, x \*/ (y /*\ z) = (x \*/ y) /*\ (x \*/ z).
-  Definition join_distributive_r_law := forall x y z, (x /*\ y) \*/ z= (x \*/ z) /*\ (y \*/ z).
-
-  (** One law implies the other three. *)
-
-  Lemma meet_distributive_l_r : meet_distributive_l_law -> meet_distributive_r_law.
-  Proof.
-  unfold meet_distributive_l_law; intro meet_distributive_l.
-  intros x y z.
-  rewrite meet_commutative.
-  rewrite meet_distributive_l.
-  rewrite meet_commutative.
-  rewrite (meet_commutative z y).
-  reflexivity.
-  Qed.
-
-  Lemma meet_distributive_r_l : meet_distributive_r_law -> meet_distributive_l_law.
-  Proof.
-  unfold meet_distributive_r_law; intro meet_distributive_r.
-  intros x y z.
-  rewrite meet_commutative.
-  rewrite meet_distributive_r.
-  rewrite meet_commutative.
-  rewrite (meet_commutative z x).
-  reflexivity.
-  Qed.
-
-  Lemma join_distributive_l_r : join_distributive_l_law -> join_distributive_r_law.
-  Proof.
-  unfold join_distributive_l_law; intro join_distributive_l.
-  intros x y z.
-  rewrite join_commutative.
-  rewrite join_distributive_l.
-  rewrite join_commutative.
-  rewrite (join_commutative z y).
-  reflexivity.
-  Qed.
-
-  Lemma join_distributive_r_l : join_distributive_r_law -> join_distributive_l_law.
-  Proof.
-  unfold join_distributive_r_law; intro join_distributive_r.
-  intros x y z.
-  rewrite join_commutative.
-  rewrite join_distributive_r.
-  rewrite join_commutative.
-  rewrite (join_commutative z x).
-  reflexivity.
-  Qed.
-
-  Lemma distributive_meet_l_join_l : meet_distributive_l_law -> join_distributive_l_law.
-  Proof.
-  unfold meet_distributive_l_law; intro meet_distributive_l.
-  intros x y z.
-  rewrite meet_distributive_l.
-  rewrite (meet_commutative (x \*/ y) x).
-  rewrite meet_absorptive.
-  rewrite (meet_distributive_l_r meet_distributive_l).
-  rewrite <- (join_associative x (x /*\ z) (y /*\ z)).
-  rewrite join_absorptive.
-  reflexivity.
-  Qed.
-
-  Lemma distributive_join_l_meet_l : join_distributive_l_law -> meet_distributive_l_law.
-  Proof.
-  unfold join_distributive_l_law; intro join_distributive_l.
-  intros x y z.
-  rewrite join_distributive_l.
-  rewrite (join_commutative (x /*\ y) x).
-  rewrite join_absorptive.
-  rewrite (join_distributive_l_r join_distributive_l).
-  rewrite <- meet_associative.
-  rewrite meet_absorptive.
-  reflexivity.
-  Qed.
-
-  Definition median_law := forall x y z,
-    (x /*\ y) \*/ (y /*\ z) \*/ (z /*\ x) = (x \*/ y) /*\ (y \*/ z) /*\ (z \*/ x).
-
-  Definition cancel_law := forall a b c, a /*\ b = c /*\ b /\ a \*/ b = c \*/ b -> a = c.
-
-  Lemma distr_cancel : meet_distributive_l_law -> cancel_law.
-  Proof.
-  unfold meet_distributive_l_law; intro meet_distributive_l.
-  intros a b c [Hi Hs].
-  rewrite <- (join_absorptive a b).
-  rewrite Hi.
-  rewrite (distributive_meet_l_join_l meet_distributive_l).
-  rewrite Hs.
-  rewrite join_commutative.
-  rewrite <- (distributive_meet_l_join_l meet_distributive_l).
-  rewrite Hi.
-  rewrite join_absorptive.
-  reflexivity.
-  Qed.
-End LatticeTheory.
-*)
